LeanNanoLlvm/Semantics/State.lean
@@ -1,6 +1,7 @@
 import LeanNanoLlvm.Semantics.Semantics
 import LeanNanoLlvm.AST.AST
 import Std.Data.ExtHashMap
+import LeanNanoLlvm.Util.Undef
 
 namespace LeanNanoLlvm.Semantics
 
@@ -29,6 +30,18 @@ structure NanoLlvmState : Type where
 
 deriving instance Inhabited for NanoLlvmState
 
-abbrev NanoLlvmStateM (retTy: Type) := StateT NanoLlvmState (Except String) retTy
+abbrev UndefChain : Type := SupplyChain Nat
+abbrev UndefState : Type := SupplyState Nat
+abbrev NanoLlvmStateM (retTy : Type) := StateT NanoLlvmState (StateT UndefState (Except String)) retTy
+
+@[simp]
+def runNanoLlvmStateM {α : Type} (m : NanoLlvmStateM α) (st : NanoLlvmState := default)
+    (uState : UndefState := default) : Except String α :=
+  ((m.run st).run uState).map (fun ((a, _), _) => a)
+
+@[simp]
+def runNanoLlvmStateMWithState {α : Type} (m : NanoLlvmStateM α) (st : NanoLlvmState := default)
+    (uState : UndefState := default) : Except String ((α × NanoLlvmState) × UndefState) :=
+  (m.run st).run uState
 
 end LeanNanoLlvm.Semantics
