LeanNanoLlvm/Util/Undef.lean
@@ -1,0 +1,34 @@
+abbrev SupplyChain (α : Type) := List α
+
+structure SupplyState (α : Type) where
+  supplyChain : SupplyChain α
+  supplyIndex : Nat
+
+abbrev UndefM (α : Type) := StateT (SupplyState α) (Except (Nat × Nat))
+
+instance [Inhabited α] : Inhabited (SupplyState α) where
+  default := ⟨[], 0⟩
+
+namespace SupplyState
+
+/-- The number of available undefined values from `s` at index `s.supplyIndex`. -/
+def isWellFormed (s : SupplyState α) : Prop :=
+  s.supplyIndex ≤ s.supplyChain.length
+
+end SupplyState
+
+namespace UndefM
+
+@[match_pattern, simp]
+def undef [Inhabited α] : UndefM α α := do
+  let s ← get
+  match s.supplyChain[s.supplyIndex]? with
+  | .some v =>
+    set { s with supplyIndex := s.supplyIndex + 1 }
+    pure v
+  | .none => throw (s.supplyIndex, s.supplyChain.length)
+
+@[match_pattern, simp]
+def value (v : α) : UndefM α α := pure v
+
+end UndefM
